Refactor & merge min/max & integer/real pow.
Co-Authored-By: Benjamin Gregoire <benjamin.gregoire@inria.fr>
Co-Authored-By: Pierre-Yves Strub <pierre-yves@strub.nu>

src/ecHiGoal.ml
@@ -1920,6 +1920,7 @@ let process_congr tc =
           (PT.pt_of_uglobal !!tc hyps LG.p_eq_iff) tc) in
       let tt1 = t_congr (o1, o2) ((List.combine a1 a2), f1.f_ty) in
       let tt2 = t_logic_trivial in
+
       FApi.t_seqs [tt0; tt1; tt2] tc
 
   | Fif (_, { f_ty = cty }, _), Fif _ ->
