theories/core/CoreInt.ec
@@ -7,7 +7,16 @@
  * -------------------------------------------------------------------- *)
 
 (* -------------------------------------------------------------------- *)
-require (*--*) Ring.
-require export Core Int Real.
-(*---*) export Ring.IntID.
+op zero   : int = 0.
+op one    : int = 1.
+op lt     : int -> int -> bool.
+op le     = fun x y => lt x y \/ x = y.
+op add    : int -> int -> int.
+op opp    : int -> int.
+op mul    : int -> int -> int.
+op absz   = fun x => (le 0 x) ? x : opp x.
 
+axiom nosmt intind (p:int -> bool):
+  (p 0) =>
+  (forall i, le 0 i => p i => p (add i 1)) =>
+  (forall i, le 0 i => p i).
